examples/riscv/kernel-trap/kernel_trap_symb_execScript.sml
@@ -1,0 +1,45 @@
+open HolKernel Parse boolLib bossLib;
+
+open wordsTheory;
+
+open bir_symbLib;
+
+open kernel_trapTheory kernel_trap_specTheory;
+
+val _ = new_theory "kernel_trap_symb_exec";
+
+(* --------------------------- *)
+(* Symbolic analysis execution *)
+(* --------------------------- *)
+
+val _ = show_tags := true;
+
+(* ---------- *)
+(* trap entry *)
+(* ---------- *)
+
+val symb_analysis_thm =
+ bir_symb_analysis_thm
+  bir_kernel_trap_prog_def
+  kernel_trap_entry_init_addr_def [kernel_trap_entry_end_addr_def]
+  bspec_kernel_trap_entry_pre_def kernel_trap_birenvtyl_def;
+
+val _ = Portable.pprint Tag.pp_tag (tag symb_analysis_thm);
+
+Theorem kernel_trap_entry_symb_analysis_thm = symb_analysis_thm
+
+(* ----------- *)
+(* trap return *)
+(* ----------- *)
+
+val symb_analysis_thm =
+ bir_symb_analysis_thm
+  bir_kernel_trap_prog_def
+  kernel_trap_return_init_addr_def [kernel_trap_return_end_addr_def]
+  bspec_kernel_trap_return_pre_def kernel_trap_birenvtyl_def;
+
+val _ = Portable.pprint Tag.pp_tag (tag symb_analysis_thm);
+
+Theorem kernel_trap_return_symb_analysis_thm = symb_analysis_thm
+
+val _ = export_theory ();
